edits on HSL.fst with Tahina

src/tls/HSL.fst
@@ -8,14 +8,18 @@ open FStar.HyperHeap
 open FStar.HyperStack
 open FStar.Ghost // after HH so as not to shadow reveal :( 
 
-/// HASH outlining how to handle incrementality and collision-resistance. No agility yet.
 
-let blocklen = 16 //unclear when to switch to machine integers
-type block = lbytes blocklen // used here both as hash tags and MAC tags
-type tag = lbytes blocklen
+(*-- HASH --*)
+//outlining how to handle incrementality and collision-resistance. No agility yet.
 
+let blocklen = 16 // unclear when to switch to machine integers; probably requires library changes.
+type block = lbytes blocklen 
+type tag = lbytes blocklen // possibly truncated; used here both as hash tags and MAC tags
+
+// core algorithm, hashing two blocks into one.
 assume val compress: block -> block -> Tot block 
 
+// injective encoding for variable-length inputs
 // supposing we add 4 bytes for the length and 1+ bytes for padding
 assume val suffix: len:nat  -> Tot (c:bytes { (len + length c) % blocklen = 0 /\ length c <= 5 /\ length c < blocklen + 5 })
 assume val block0: block 
@@ -33,14 +37,12 @@ let hash b = hash2 block0 (b @| suffix (length b))
 
 type accv = | Acc: len:nat -> a:block -> b:lbytes (len % blocklen) -> accv 
 
-// partial computation (specification) 
+// incremental computation (specification) 
 val hashA: bytes -> Tot accv
 let hashA b = 
   let pending = length b % blocklen in 
   let hashed, rest = split b (length b - pending) in
   Acc (length b) (hash2 block0 hashed) rest
-
-//type acc = content:bytes (* TODO: ghost in real mode *) & v:accv { v = hashA content }
 
 let start = hashA empty_bytes // i.e. block0
 
@@ -51,12 +53,25 @@ val extend:
   b:bytes ->
   Tot (a:accv { a == hashA (content @| b) })
 
-assume val hash2_append:
+assume val split_append: xs:bytes -> ys:bytes -> i:nat { i <= Seq.length xs } -> 
+  Lemma(
+    let c,b = split xs i in (split (xs@|ys) i == (c, (b@|ys))))
+  
+val hash2_append:
   a:block -> 
   b0:bytes { length b0 % blocklen = 0 } -> 
   b1:bytes { length b1 % blocklen = 0 } -> 
-  Lemma (hash2 a (b0 @| b1) = hash2 (hash2 a b0) b1)
-
+  Lemma (ensures hash2 a (b0 @| b1) == hash2 (hash2 a b0) b1) (decreases (length b0))
+let rec hash2_append a b0 b1 = 
+  if length b0 = 0 then (
+    assert(Seq.equal b0 empty_bytes);
+    assert(Seq.equal (b0 @| b1) b1);
+    assert_norm(hash2 a empty_bytes == a))
+  else 
+    let c,b = split b0 blocklen in
+    split_append b0 b1 blocklen; 
+    hash2_append (compress a c) b b1
+  
 let extend content v b = 
   let z = v.b @| b in 
   let pending = length z % blocklen in
@@ -79,7 +94,13 @@ let extend content v b =
   Acc (v.len + length b) (hash2 v.a hashed) rest
 
 // witnessing that we hashed this particular content (for collision detection)
-assume val hashed: bytes -> Type
+// to be replaced by a witness of inclusion in a global table of all hash computations.
+// (not sure how to manage that table)
+assume val hashed: bytes -> Type 
+
+// Hash.table: strong invariants: hash is injective on its contents.
+// witnessed(fun h -> sel h Hash.table `contains` b)
+
 val finalize: 
   content:bytes (* TODO: ghost in real mode *) ->
   a:accv { a = hashA content } -> 
@@ -89,9 +110,8 @@ val finalize:
     t = hash content /\ 
     hashed content /\
     h0 == h1 
-    // to be adjusted, e.g. 
-    // modifies_one h0 h1 hashTable /\ 
-    //sel h1 hashTable == snoc (sel h0 hashTable) (content, t)
+    // TBC, e.g. 
+    // modifies_one h0 h1 hashTable /\ sel h1 hashTable == snoc (sel h0 hashTable) (content, t)
   ))
 
 let finalize content v = 
@@ -104,31 +124,53 @@ let finalize content v =
   hash2_append block0 b0 b1; 
   hash2 v.a b1
 
+(*
+val collision_resistant: c0: bytes -> c1: bytes { hashed c0 /\ hashed c1 } -> ST unit 
+  (requires (fun h0 -> True))
+  (ensures (hash c0 = hash c1 ==> c0 = c1))
+let collision_resistant c0 c1 =
+  testify(hashed c0);
+  testify(hashed c1);
+  let current = !Hash.table in 
+  ()
+*)
 
-///// From Handshake.Msg
+
+
+(*-- Handshake.Msg --*) 
+// simplified handshake messages; for this outline we show that the client 
+// agrees with the server on the two offers after checking the Finished message
 
 assume type offer: Type0
 // 17-01-19 Still confused about concrete syntax for universes + eqtypes
 noeq type msg: Type0 = | ClientHello of offer | ServerHello of offer | Finished of tag
-// simplified handshake message; for this outline we show that the client agrees with the server on the two offers after checking the Finished message
 
 assume val format: msg -> Tot bytes 
-// TODO formatting is injective
-
 assume val parse_msg: b:bytes -> Tot (option (m:msg {b = format m}))
 assume val tagged: msg -> Tot bool // do we compute a hash of the transcript ending with this message?
 assume val eoflight: msg -> Tot bool // does this message complete the flight? 
 
-///// An outline of HSL 
+
+
+
+
+
+
+///// An outline of HandshakeLog
 
 let transcript_bytes ms = List.Tot.fold_left (fun a m -> a @| format m) empty_bytes ms
 // we will need to prove it is injective, we will rely in turn on concrete msg formats
+
+// formatting of the whole transcript is injective (what about binders?)
+assume val transcript_format_injective: ms0:list msg -> ms1:list msg -> 
+  Lemma(Seq.equal (transcript_bytes ms0) (transcript_bytes ms1) ==> ms0 == ms1)
 
 //17-01-23  how to prove this from the definition above??
 assume val transcript_bytes_append: ms0: list msg -> ms1: list msg -> 
   Lemma (transcript_bytes (ms0 @ ms1) = transcript_bytes ms0 @| transcript_bytes ms1)
 
-// a specification of the hashed-prefix tags required for a given flight 
+
+// full specification of the hashed-prefix tags required for a given flight 
 val tags: prior: list msg -> incoming: list msg -> Tot (list tag) (decreases incoming) 
 let rec tags prior incoming = 
   match incoming with 
@@ -145,7 +187,14 @@ val tags_nil_nil: prior: list msg -> Lemma (tags prior [] = [])
 let tags_nil_nil prior = ()
 
 //17-01-23 plausible ? 
-assume val tags_append: prior: list msg -> in0: list msg -> in1: list msg -> Lemma(tags prior (in0 @ in1) = tags prior in0 @ tags (prior @ in0) in1)
+assume val tags_append: prior: list msg -> in0: list msg -> in1: list msg -> 
+  Lemma(tags prior (in0 @ in1) == tags prior in0 @ tags (prior @ in0) in1)
+(*
+let rec tags_append prior in0 in1 = 
+  match in0 with
+  | [] -> ( assert(prior @ in0 == prior) )
+  | m :: ms -> ...
+*)      
 
 
 (* STATE *)
@@ -161,6 +210,11 @@ noeq type state = | State:
   state
 type t = r:ref state // 17-01-19 HS naming!?
 
+val transcripT: h:mem -> t -> GTot (list msg) // the current transcript shared with the handshake
+let transcripT h (r:t) = (FStar.HyperStack.sel h r).transcript
+
+(*
+
 (*
 // type flight (prior:erased (list msg)) = ms:list msg & hs:list tag { hs = tags (reveal prior) ms }
 
@@ -174,13 +228,9 @@ abstract type state = State
   hash: Hash.t { hash = HashA (transcript_bytes (List.Tot.append transcript input_msgs)) } // current hash state
 *)
 
-val transcripT: h:mem -> t -> GTot (list msg) // the current transcript shared with the handshake
-let transcripT h (r:t) = 
-  let s = FStar.HyperStack.sel h r in 
-  s.transcript
-
-(*
-We will also need to keep track of lengths in the input/output buffers To separate between Reading and Writing modes, a precondition for sending a message should be that both input_bytes and input_msgs are empty.(unclear who should check for emptyset, and how to react to extra bytes buffered past the input flight)
+We will also need to keep track of lengths in the input/output buffers
+To separate between Reading and Writing modes, a precondition for sending a message should be that both input_bytes and input_msgs are empty. 
+(unclear who should check for emptyset, and how to react to extra bytes buffered past the input flight)
 *)
 
 (* commenting out the rest of the outline not used in the sample code for now: 
@@ -224,29 +274,37 @@ let receive r bs =
   match parse_msg bs with // assuming bs is a potential whole message
   | None -> None
   | Some m -> (
-      let State transcript ms hs a = !r in
-      let content0 = transcript_bytes (transcript @ ms) in 
-      let content1 = transcript_bytes ((transcript @ ms) @ [m]) in 
-      transcript_bytes_append (transcript @ ms) [m];
-      assert(hs = tags transcript ms); 
-      tags_append transcript ms [m];
-      let ms = ms @ [m]  in
+      let State prior ms hs a = !r in
+      let content0 = transcript_bytes (prior @ ms) in 
+      let content1 = transcript_bytes (prior @ (ms @ [m])) in 
+      //let content1 = transcript_bytes ((transcript @ ms) @ [m]) in 
+      assume((prior @ ms) @ [m] == prior @ (ms @ [m])); //17-01-24 dubious
+      transcript_bytes_append prior ms;
+      transcript_bytes_append prior (ms@[m]);
+      transcript_bytes_append (prior@ms) [m];
+      assert(Seq.equal content1 (content0 @| transcript_bytes [m]));
       assert_norm(Seq.equal (transcript_bytes [m]) (format m));
       assert(Seq.equal content1 (content0 @| format m));
+      assert(hs = tags prior ms); 
+      tags_append prior ms [m];
+      let ms = ms @ [m]  in
+      assert_norm(Seq.equal (transcript_bytes [m]) (format m));
       let a = extend content0 a bs in
       assert(a == hashA content1);
-      let hs : hs: list tag { hs = tags transcript ms } = 
+      let hs : hs: list tag { hs == tags prior ms } = 
         if tagged m 
-          then (hs @ [finalize content1 a]) 
-          else [] in 
+          then (
+            hs @ [finalize content1 a]) 
+          else 
+            hs in 
       if eoflight m then  
-        let transcript = transcript @ ms in 
-        ( tags_nil_nil transcript; 
-          assert(a == hashA (transcript_bytes transcript));
-          r := State transcript [] [] a; 
+        let prior1 = prior @ ms in 
+        ( tags_nil_nil prior; 
+          assert(a == hashA (transcript_bytes prior1));
+          r := State prior1 [] [] a; 
           Some (ms,hs) ) 
       else (
-        r := State transcript ms hs a; 
+        r := State prior ms hs a; 
         None ))
 
 
@@ -256,7 +314,9 @@ design: how to return flights with intermediate tags?
 TODO: support multiple epochs? 
 *)
 
-////// An outline of HS 
+
+
+////// An outline of Handshake
 
 assume val nego: offer -> GTot offer // the server's choice of parameters
 assume val mac_verify: h:tag -> t:tag -> 
@@ -267,7 +327,7 @@ let inj_format c0 s0 c1 s1 : Lemma (
   hash (format (ClientHello c1) @| format (ServerHello s1)) ==> c0 == c1 /\ s0 == s1 ) = 
   assume false
 
-
+// the HS handler for receiving the server flight after sending a client offer
 val process: log:t -> bytes -> c:offer -> ST (option offer)
   (requires (fun h0 -> transcripT h0 log == [ClientHello c]))
   (ensures (fun h0 o h1 -> 
@@ -278,8 +338,8 @@ let process log (raw:bytes) client_offer =
   match receive log raw with 
   | Some ([ServerHello server_offer; Finished tag], [hash_ch_sh]) -> 
     if mac_verify hash_ch_sh tag then  (
-    assert(hash_ch_sh = hash (format (ClientHello client_offer) @| format (ServerHello (server_offer)))); 
-    assert(exists offer.  hash_ch_sh == hash (format (ClientHello offer) @| format (ServerHello (nego offer))));
+    assert(hash_ch_sh = hash(transcript_bytes [ ClientHello client_offer; ServerHello server_offer])); 
+    assert(exists offer.  hash_ch_sh == hash(transcript_bytes[ ClientHello offer; ServerHello (nego offer)]));
     assert(server_offer == nego client_offer);
     assume false;
     Some server_offer 
